coq/Relations_ext.v
@@ -14,19 +14,19 @@ Notation "[ * R ]" :=
 
 Hint Resolve rt1n_refl.
 
-Lemma rt1n_trans' : forall A R, transitive A [* R].
+Lemma rtc_trans' : forall A R, transitive A [* R].
 Proof.
   move => A R t1 t2 t3.
   rewrite -!clos_rt_rt1n_iff.
   apply rt_trans.
 Qed.
 
-Lemma rt1n_step : forall (A : Set) (R : relation A), inclusion R [* R].
+Lemma rtc_step : forall (A : Set) (R : relation A), inclusion R [* R].
 Proof.
   move => A R x y H; apply rt1n_trans with y; auto.
 Qed.
 
-Lemma clos_rt_map :
+Lemma rtc_map :
   forall A (R R' : relation A), inclusion R R' -> inclusion [* R] [* R'].
 Proof.
   move => A R R' H.
@@ -34,15 +34,15 @@ Proof.
   apply rt1n_trans with t2; auto.
 Qed.
 
-Lemma rt1n_nest_elim : forall A (R : relation A), same_relation [* [* R]] [* R].
+Lemma rtc_nest_elim : forall A (R : relation A), same_relation [* [* R]] [* R].
 Proof.
   move => A R t1 t2; split.
   - move: t1 t2; refine (clos_refl_trans_1n_ind A _ _ _ _) => //.
-    by move => t1 t2 t3 H _ H0; apply rt1n_trans' with t2.
+    by move => t1 t2 t3 H _ H0; apply rtc_trans' with t2.
   - apply clos_rt1n_step.
 Qed.
 
-Lemma rt1n_semi_confluent :
+Lemma rtc_semi_confluent :
   forall A (R S : relation A),
   (forall t1 t2 t3, R t1 t2 -> S t1 t3 -> exists t4, S t2 t4 /\ R t3 t4) ->
   (forall t1 t2 t3, [* R] t1 t2 -> S t1 t3 ->
@@ -57,25 +57,25 @@ Proof.
     by apply rt1n_trans with t3'.
 Qed.
 
-Lemma rt1n_confluent :
+Lemma rtc_confluent :
   forall A (R : relation A), confluent R -> confluent [* R].
 Proof.
   move => A R H.
-  apply rt1n_semi_confluent.
-  move: (rt1n_semi_confluent R H) => {H} H t1 t2 t3 H0 H1.
+  apply rtc_semi_confluent.
+  move: (rtc_semi_confluent R H) => {H} H t1 t2 t3 H0 H1.
   by case: (H t1 t3 t2 H1 H0) => t4; case => H2 H3; exists t4.
 Qed.
 
-Lemma rt1n_confluent' : forall A (R R' : relation A),
+Lemma rtc_confluent' : forall A (R R' : relation A),
   inclusion R R' -> inclusion R' [* R] -> confluent R' -> confluent [* R].
 Proof.
   move => A R R' H H0 H1 t1 t2 t3 H2 H3.
-  case (rt1n_confluent H1 (clos_rt_map _ H H2) (clos_rt_map _ H H3))
+  case (rtc_confluent H1 (rtc_map _ H H2) (rtc_map _ H H3))
     => t4 [? ?].
-  by exists t4; split; rewrite -rt1n_nest_elim; apply (clos_rt_map _ H0).
+  by exists t4; split; rewrite -rtc_nest_elim; apply (rtc_map _ H0).
 Qed.
 
-Theorem rt1n_preservation :
+Theorem rtc_preservation :
   forall A (P : A -> Prop) (R : relation A),
   (forall x y, R x y -> P x -> P y) -> forall x y, [* R] x y -> P x -> P y.
 Proof.
